add implications to vmprop_zero for logrel_prim

theories/logrel/logrel.v
@@ -22,6 +22,43 @@ Section logrel.
 
   (** definitions **)
 
+   (* [transaction_pagetable_entries_transferred] : For donation, the half of transaction entries that are kept by sender in case
+      of sharing and lending are also be passed around between the sender and the receiver, as retrieval in this case also requires
+      full entries.
+      Pagetable entries are transferred along as both sender and receiver could be the exclusive owner of those pages. *)
+  Definition transaction_pagetable_entries_transferred i (trans: gmap Addr transaction) : iProp Σ:=
+    big_sepFM trans (λ kv, kv.2.1.2 = Donation ∧ (kv.2.1.1.1.2 = i ∨ kv.2.1.1.1.1 = i)) (λ k v, k -{1/2}>t v.1 ∗ pgt v.1.1.2 1 v.1.1.1.1 true)%I.
+
+  (* [retrieval entries]: half of all retrieval entries of i-related transactions are required.
+     For transactions where i is the sender, we need the corresponding retrieval entries to check if it is allowed for i to reclaim,
+     for the cases when i is the receiver, they are required so that i can retrieve or relinquish *)
+  (* There are also some cases when we need the second half, as in those cases we may update/remove the retrival state *)
+  (* XXX: How to relate retrieval and transaction entries? Using option(frac_agree transaction,option bool)? or is it unnecessary? *)
+  Definition retrieval_entries_transferred i (trans: gmap Addr transaction) : iProp Σ:=
+    (big_sepFM trans (λ kv, kv.2.1.1.1.2 = i ∨ kv.2.1.1.1.1 = i) (λ k v, k -{1/2}>re v.2 )%I) ∗
+    (big_sepFM trans (λ kv, (kv.2.1.1.1.1 = i ∨ kv.2.1.1.1.2 = i) ∧ kv.2.2 = false) (λ k v, k -{1/2}>re v.2)%I).
+
+  (* [transaction_pagetable_entries_owned]: transaction and page table entries that are owned initially by i,
+     i.e. they are not transferred by VMProp, so we doesn't need to take care of them when reasoning the primary VM.
+     As the invoker of sharing and lending transactions, i always has the ownership of involved pages.
+     Therefore, i ownes these pagetable entries even if they are in some transactions.
+     Furthermore, since it is suffice for the receiver to retrieve or relinquish with half of transacitons entries,
+     while the sender needs full to reclaim, we let i always own half and only pass the otner half around with VMProp*)
+  (* [TODO] relation to [pagetable_entries_excl_owned] *)
+  Definition transaction_pagetable_entries_owned i (trans: gmap Addr transaction) : iProp Σ:=
+    big_sepFM trans (λ kv, kv.2.1.1.1.1 = i ∧ kv.2.1.2 ≠ Donation) (λ k v, k -{1/2}>t v.1 ∗ pgt v.1.1.2 1 v.1.1.1.1 (bool_decide (v.1.2 ≠ Sharing)))%I.
+
+  (* [TODO] *)
+  Definition retrieval_entries_owned i (trans: gmap Addr transaction) : iProp Σ:=
+    (big_sepFM trans (λ kv, kv.2.1.1.1.2 = i ∧ kv.2.2 = true) (λ k v, k -{1/2}>re v.2)%I).
+
+  Definition transaction_pagetable_entries_transferred_except (i: VMID) (trans: gmap Addr transaction) : iProp Σ:=
+    big_sepFM trans (λ kv, kv.2.1.2 = Donation ∧ ¬(kv.2.1.1.1.2 = i ∨ kv.2.1.1.1.1 = i)) (λ k v, k -{1/2}>t v.1 ∗ pgt v.1.1.2 1 v.1.1.1.1 true)%I.
+
+  Definition retrieval_entries_transferred_except (i: VMID) (trans: gmap Addr transaction) : iProp Σ:=
+    (big_sepFM trans (λ kv, ¬(kv.2.1.1.1.2 = i ∨ kv.2.1.1.1.1 = i)) (λ k v, k -{1/2}>re v.2 )%I) ∗
+    (big_sepFM trans (λ kv, ¬(kv.2.1.1.1.2 = i ∨ kv.2.1.1.1.1 = i) ∧ kv.2.2 = false) (λ k v, k -{1/2}>re v.2)%I).
+
   Context (i : (leibnizO VMID)).
 
   Program Definition interp_execute: iPropO Σ :=
@@ -37,35 +74,6 @@ Section logrel.
   Definition transaction_hpool_global_transferred (trans: gmap Addr transaction) : iProp Σ:=
     ∃ hpool,  ⌜hpool ∪ dom (gset _ ) trans = hs_all⌝ ∗ fresh_handles 1 hpool ∗ ⌜trans_ps_disj trans⌝ ∗ [∗ map] h ↦ tran ∈ trans, h -{1/2}>t tran.1.
 
-  (* [transaction_pagetable_entries_owned]: transaction and page table entries that are owned initially by i,
-     i.e. they are not transferred by VMProp, so we doesn't need to take care of them when reasoning the primary VM.
-     As the invoker of sharing and lending transactions, i always has the ownership of involved pages.
-     Therefore, i ownes these pagetable entries even if they are in some transactions.
-     Furthermore, since it is suffice for the receiver to retrieve or relinquish with half of transacitons entries,
-     while the sender needs full to reclaim, we let i always own half and only pass the otner half around with VMProp*)
-  (* [TODO] relation to [pagetable_entries_excl_owned] *)
-  Definition transaction_pagetable_entries_owned (trans: gmap Addr transaction) : iProp Σ:=
-    big_sepFM trans (λ kv, kv.2.1.1.1.1 = i ∧ kv.2.1.2 ≠ Donation) (λ k v, k -{1/2}>t v.1 ∗ pgt v.1.1.2 1 v.1.1.1.1 (bool_decide (v.1.2 ≠ Sharing)))%I.
-
-   (* [transaction_pagetable_entries_transferred] : For donation, the half of transaction entries that are kept by sender in case
-      of sharing and lending are also be passed around between the sender and the receiver, as retrieval in this case also requires
-      full entries.
-      Pagetable entries are transferred along as both sender and receiver could be the exclusive owner of those pages. *)
-  Definition transaction_pagetable_entries_transferred (trans: gmap Addr transaction) : iProp Σ:=
-    big_sepFM trans (λ kv, kv.2.1.2 = Donation ∧ (kv.2.1.1.1.2 = i ∨ kv.2.1.1.1.1 = i)) (λ k v, k -{1/2}>t v.1 ∗ pgt v.1.1.2 1 v.1.1.1.1 true)%I.
-
-  (* [retrieval entries]: half of all retrieval entries of i-related transactions are required.
-     For transactions where i is the sender, we need the corresponding retrieval entries to check if it is allowed for i to reclaim,
-     for the cases when i is the receiver, they are required so that i can retrieve or relinquish *)
-  (* There are also some cases when we need the second half, as in those cases we may update/remove the retrival state *)
-  (* XXX: How to relate retrieval and transaction entries? Using option(frac_agree transaction,option bool)? or is it unnecessary? *)
-  Definition retrieval_entries_transferred(trans: gmap Addr transaction) : iProp Σ:=
-    (big_sepFM trans (λ kv, kv.2.1.1.1.2 = i ∨ kv.2.1.1.1.1 = i) (λ k v, k -{1/2}>re v.2 )%I) ∗
-    (big_sepFM trans (λ kv, (kv.2.1.1.1.1 = i ∨ kv.2.1.1.1.2 = i) ∧ kv.2.2 = false) (λ k v, k -{1/2}>re v.2)%I).
-
-  (* [TODO] *)
-  Definition retrieval_entries_owned(trans: gmap Addr transaction) : iProp Σ:=
-    (big_sepFM trans (λ kv, kv.2.1.1.1.2 = i ∧ kv.2.2 = true) (λ k v, k -{1/2}>re v.2)%I).
 
   (* [memory_transferred]: some memory points-to predicates are transferred by VMProp.
      the memory is the memory of pages associated with a transaction and i has or may have access to. *)
@@ -86,8 +94,8 @@ Section logrel.
     (R0 @@ V0 ->r encode_hvc_func(Send) ∗ (∃ rx_state'', RX_state@ i := rx_state'') ∗ ∃ j p_rx l, ⌜j ≠ i⌝ ∗ RX@ j := p_rx ∗ RX_state{1/2}@j := Some(l,i)
                           ∗ (∃r1, R1 @@ V0 ->r r1 ∗ ⌜decode_vmid r1 = Some j⌝) ∗  R2 @@ V0 ->r l ∗ ∃ mem_rx, memory_page p_rx mem_rx).
 
-  Definition vmprop_zero_pre (Ψ: PID -d> PID -d> (gmap Word transaction) -d> iPropO Σ) :PID -d> PID -d> iPropO Σ :=
-    λ p_tx p_rx, (∃ ps_na'' ps_acc'' trans'' ,
+  Definition vmprop_zero_pre (Ψ: PID -d> PID -d> (gmap Word transaction) -d> iPropO Σ) :PID -d> PID -d> (gmap Word transaction) -d> iPropO Σ :=
+    λ p_tx p_rx trans', (∃ ps_na'' ps_acc'' trans'' ,
                            let ps_macc_trans'' := pages_in_trans (trans_memory_in_trans trans'') in
                            (* lower bound *)
                            i -@{1/2}A> ps_acc'' ∗
@@ -95,8 +103,8 @@ Section logrel.
                            ⌜ps_na'' ## ps_acc'' ∪ ps_macc_trans''⌝ ∗
                            (* transaction and pagetable entries *)
                            transaction_hpool_global_transferred trans'' ∗
-                           transaction_pagetable_entries_transferred trans'' ∗
-                           retrieval_entries_transferred trans'' ∗
+                           transaction_pagetable_entries_transferred i trans'' ∗
+                           retrieval_entries_transferred i trans'' ∗
                            (* memory *)
                            (∃ mem_trans, memory_pages ps_macc_trans'' mem_trans) ∗
                            (* status of RX *)
@@ -104,6 +112,10 @@ Section logrel.
                            rx_page i p_rx ∗ (∃ mem_rx, memory_page p_rx mem_rx) ∗
                            rx_pages ((list_to_set (list_of_vmids)) ∖ {[i]}) ∗
                            return_reg_rx i ∗
+                           (* implications *)
+                           (transaction_pagetable_entries_transferred_except i trans' -∗ transaction_pagetable_entries_transferred_except i trans'') ∗
+                           (retrieval_entries_transferred_except i trans' -∗ retrieval_entries_transferred_except i trans'') ∗
+                           (transaction_pagetable_entries_owned V0 trans' -∗ transaction_pagetable_entries_transferred V0 trans'') ∗
                            VMProp i (Ψ p_tx p_rx trans'') (1/2)%Qp)%I.
 
   Definition vmprop_unknown_pre
@@ -125,8 +137,8 @@ Section logrel.
                (* we can derive ⌜{[p_rx;p_tx]} ## ps_mem_in_trans''⌝ from rx_page/tx_page ∗ transaction_hpool_global_transferred *)
                (* transaction and pagetable entries *)
                transaction_hpool_global_transferred trans' ∗
-               transaction_pagetable_entries_transferred trans' ∗
-               retrieval_entries_transferred trans' ∗
+               transaction_pagetable_entries_transferred i trans' ∗
+               retrieval_entries_transferred i trans' ∗
                (* memory *)
                (∃ mem_trans, memory_transferred trans' mem_trans) ∗
                R0 @@ V0 ->r encode_hvc_func(Run) ∗ R1 @@ V0 ->r encode_vmid(i) ∗ (∃ r2, R2 @@ V0 ->r r2) ∗
@@ -146,13 +158,13 @@ Section logrel.
                 in a concrete example(as we give a concrete [trans] at the first and can reason about what should be the
                 [trans'] that satisfies the relation as we know the behaviors of VMs) than in a general case. So we leave
                 the proofs to the users of LR. *)
-               (transaction_pagetable_entries_owned trans -∗ transaction_pagetable_entries_owned trans') ∗
+               (transaction_pagetable_entries_owned i trans -∗ transaction_pagetable_entries_owned i trans') ∗
                (pagetable_entries_excl_owned i ps_oea -∗ pagetable_entries_excl_owned i ps_oea') ∗
-               (retrieval_entries_owned trans -∗ retrieval_entries_owned trans') ∗
+               (retrieval_entries_owned i trans -∗ retrieval_entries_owned i trans') ∗
                ((∃ mem_oea, memory_pages ps_oea mem_oea) ∗ (∃ mem_trans, memory_transferred trans' mem_trans) -∗
                 ∃ mem_all, memory_pages (ps_acc' ∖ {[p_rx;p_tx]} ∪ ps_macc_trans') mem_all) ∗
                (* if i yielding, we give following resources back to pvm *)
-               VMProp V0 (vmprop_zero_pre Φ p_tx p_rx) (1/2)%Qp)%I.
+               VMProp V0 (vmprop_zero_pre Φ p_tx p_rx trans') (1/2)%Qp)%I.
 
   Local Instance vmprop_unknown_pre_contractive : Contractive (vmprop_unknown_pre).
   Proof.
@@ -167,7 +179,7 @@ Section logrel.
     rewrite /VMProp.
     repeat f_equiv.
     apply Hvmprop_unknown.
-Qed.
+  Qed.
 
   Definition vmprop_unknown:= fixpoint (vmprop_unknown_pre).
 
@@ -184,20 +196,20 @@ Qed.
           LB@ i := [ps_na'] ∗
           ⌜ps_na' ## ps_acc' ∪ ps_macc_trans'⌝ ∗
           transaction_hpool_global_transferred trans' ∗
-          transaction_pagetable_entries_transferred trans' ∗
-          retrieval_entries_transferred trans' ∗
+          transaction_pagetable_entries_transferred i trans' ∗
+          retrieval_entries_transferred i trans' ∗
           (∃ mem_trans, memory_transferred trans' mem_trans) ∗
           R0 @@ V0 ->r encode_hvc_func(Run) ∗ R1 @@ V0 ->r encode_vmid(i) ∗ (∃ r2, R2 @@ V0 ->r r2) ∗
           RX_state@ i := rx_state ∗
           (rx_page i p_rx) ∗
           (∃ mem_rx, memory_page p_rx mem_rx) ∗
           rx_pages (list_to_set (list_of_vmids) ∖ {[i]}) ∗
-          (transaction_pagetable_entries_owned trans -∗ transaction_pagetable_entries_owned trans') ∗
+          (transaction_pagetable_entries_owned i trans -∗ transaction_pagetable_entries_owned i trans') ∗
           (pagetable_entries_excl_owned i ps_oea -∗ pagetable_entries_excl_owned i ps_oea') ∗
-          (retrieval_entries_owned trans -∗ retrieval_entries_owned trans') ∗
+          (retrieval_entries_owned i trans -∗ retrieval_entries_owned i trans') ∗
           ((∃ mem_oea, memory_pages ps_oea mem_oea) ∗ (∃ mem_trans, memory_transferred trans' mem_trans) -∗
           ∃ mem_all, memory_pages (ps_acc' ∖ {[p_rx;p_tx]} ∪ ps_macc_trans') mem_all) ∗
-          VMProp V0 (vmprop_zero p_tx p_rx) (1/2)%Qp)%I.
+          VMProp V0 (vmprop_zero p_tx p_rx trans') (1/2)%Qp)%I.
   Proof.
     rewrite /vmprop_unknown //.
     rewrite (fixpoint_unfold vmprop_unknown_pre).
@@ -216,21 +228,21 @@ Qed.
                i -@{1/2}A> ps_acc' ∗
                LB@ i := [ps_na'] ∗
                ⌜ps_na' ## ps_acc' ∪ ps_macc_trans'⌝ ∗
-               transaction_hpool_global_transferred trans' ∗
-               transaction_pagetable_entries_transferred trans' ∗
-               retrieval_entries_transferred trans' ∗
+               transaction_hpool_global_transferred  trans' ∗
+               transaction_pagetable_entries_transferred i trans' ∗
+               retrieval_entries_transferred i trans' ∗
                (∃ mem_trans, memory_transferred trans' mem_trans) ∗
                R0 @@ V0 ->r encode_hvc_func(Run) ∗ R1 @@ V0 ->r encode_vmid(i) ∗ (∃ r2, R2 @@ V0 ->r r2) ∗
                RX_state@ i := rx_state ∗
                (rx_page i p_rx) ∗
                (∃ mem_rx, memory_page p_rx mem_rx) ∗
                rx_pages (list_to_set (list_of_vmids) ∖ {[i]}) ∗
-               (transaction_pagetable_entries_owned trans -∗ transaction_pagetable_entries_owned trans') ∗
+               (transaction_pagetable_entries_owned i trans -∗ transaction_pagetable_entries_owned i trans') ∗
                (pagetable_entries_excl_owned i ps_oea -∗ pagetable_entries_excl_owned i ps_oea') ∗
-               (retrieval_entries_owned trans -∗ retrieval_entries_owned trans') ∗
+               (retrieval_entries_owned i trans -∗ retrieval_entries_owned i trans') ∗
                ((∃ mem_oea, memory_pages ps_oea mem_oea) ∗ (∃ mem_trans, memory_transferred trans' mem_trans) -∗
                 ∃ mem_all, memory_pages (ps_acc' ∖ {[p_rx;p_tx]} ∪ ps_macc_trans') mem_all) ∗
-               VMProp V0 (vmprop_zero p_tx p_rx) (1/2)%Qp)%I.
+               VMProp V0 (vmprop_zero p_tx p_rx trans') (1/2)%Qp)%I.
     Proof.
       rewrite /vmprop_unknown.
       (* be patient, this line takes 30+ sec.. *)
@@ -250,8 +262,8 @@ Qed.
       i -@{1/2}A> ps_acc ∗
       ⌜{[p_tx;p_rx]} ⊆ ps_acc⌝ ∗
       pagetable_entries_excl_owned i ps_oea ∗
-      transaction_pagetable_entries_owned trans ∗
-      retrieval_entries_owned trans ∗
+      transaction_pagetable_entries_owned i trans ∗
+      retrieval_entries_owned i trans ∗
       (∃ mem_oea, memory_pages ps_oea mem_oea) ∗
       VMProp i (vmprop_unknown p_tx p_rx trans) (1/2)%Qp
     )%I.
@@ -271,12 +283,6 @@ Section logrel_prim.
     (big_sepFM trans (λ kv, True) (λ k v, k -{1/2}>re v.2 )%I) ∗
     (big_sepFM trans (λ kv, kv.2.2 = false) (λ k v, k -{1/2}>re v.2)%I).
 
-  Definition transaction_pagetable_entries_transferred_except (i: VMID) (trans: gmap Addr transaction) : iProp Σ:=
-    big_sepFM trans (λ kv, kv.2.1.2 = Donation ∧ ¬(kv.2.1.1.1.2 = i ∨ kv.2.1.1.1.1 = i)) (λ k v, k -{1/2}>t v.1 ∗ pgt v.1.1.2 1 v.1.1.1.1 true)%I.
-
-  Definition retrieval_entries_transferred_except (i: VMID) (trans: gmap Addr transaction) : iProp Σ:=
-    (big_sepFM trans (λ kv, ¬(kv.2.1.1.1.2 = i ∨ kv.2.1.1.1.1 = i)) (λ k v, k -{1/2}>re v.2 )%I) ∗
-    (big_sepFM trans (λ kv, ¬(kv.2.1.1.1.2 = i ∨ kv.2.1.1.1.1 = i) ∧ kv.2.2 = false) (λ k v, k -{1/2}>re v.2)%I).
 
   Program Definition interp_access_prim p_tx p_rx ps_acc trans rx_state: iPropO Σ:=
     (
